Splinter/Journal/Bundle.i.dfy
@@ -1,2 +1,3 @@
 include "../CoordinationLayer/Bundle.i.dfy"
 include "PagedJournalRefinement.i.dfy"
+include "LinkedJournal.i.dfy"
